A.fst
@@ -1,0 +1,24 @@
+module A
+
+let a0 = 0
+let a1 = 1
+let a2 = 2
+let a3 = 3
+let a4 = 4
+let a5 = 5
+let a6 = 6
+let a7 = 7
+let a8 = 8
+let a9 = 9
+
+type t0 = | T0A | T0B | T0C
+type t1 = | T1A | T1B | T1C
+type t2 = | T2A | T2B | T2C
+type t3 = | T3A | T3B | T3C
+type t4 = | T4A | T4B | T4C
+type t5 = | T5A | T5B | T5C
+type t6 = | T6A | T6B | T6C
+type t7 = | T7A | T7B | T7C
+type t8 = | T8A | T8B | T8C
+type t9 = | T9A | T9B | T9C
+
