B.fst
@@ -1,0 +1,7 @@
+module B
+
+// open A
+open A (a1, a2)
+
+let _ = a1
+
